Revised the proof strategy for relations and factored it into a separate file. In terms of the model, I decided to opt for the solution that keeps the dashed variables constant rather than closing the relational binding set. This proved to introduce less complications into proofs. The work on the relational proof strategy is now fairly polished; the features that are missing are support for quantifiers, substitution, and the proof that the simplified version of the definition for sequential composition is equivalent to the algebraic one.

theories/generic/utp_rel.thy
@@ -7,30 +7,33 @@
 header {* Relations *}
 
 theory utp_rel
-imports utp_pred utp_eval utp_subst
+imports utp_pred utp_subst
 begin
-
-subsection {* Type Synonyms *}
-
-type_synonym ('VALUE, 'TYPE) RELATION =
-  "(('VALUE, 'TYPE) BINDING \<times> ('VALUE, 'TYPE) BINDING) set"
 
 context PRED
 begin
 
-subsection {* Sequential Composition *}
+subsection {* Restrictions *}
 
-definition OTHER_VAR :: "'TYPE VAR set" where
-"OTHER_VAR = VAR - (DASHED \<union> UNDASHED)"
+definition NON_REL_VAR :: "'TYPE VAR set" where
+"NON_REL_VAR = VAR - (DASHED \<union> UNDASHED)"
 
-definition COMPOSABLE :: "('VALUE, 'TYPE) RELATION" where
+definition COMPOSABLE ::
+  "(('VALUE, 'TYPE) BINDING \<times>
+    ('VALUE, 'TYPE) BINDING) set" where
 "COMPOSABLE = {(b1, b2) .
-   (\<forall> v \<in> UNDASHED . b1(dash v) = b2 v) \<and> b1 \<cong> b2 on OTHER_VAR}"
+   (\<forall> v \<in> UNDASHED . b1(dash v) = b2 v) \<and> b1 \<cong> b2 on NON_REL_VAR}"
 
-definition SS :: "'TYPE VAR \<Rightarrow> 'TYPE VAR" where
-"SS = (\<lambda> v .
-   if v \<in> UNDASHED then (dash v) else
-   if v \<in> DASHED then (undash v) else v)"
+subsection {* Operators *}
+
+subsubsection {* Skip *}
+
+definition SkipR :: "('VALUE, 'TYPE) PREDICATE" where
+"SkipR = {b \<in> WF_BINDING . \<forall> v \<in> UNDASHED . b v = b (dash v)}"
+
+notation SkipR ("II")
+
+subsubsection {* Sequential Composition *}
 
 definition SemiR ::
   "('VALUE, 'TYPE) PREDICATE \<Rightarrow>
@@ -45,80 +48,16 @@ definition SemiR ::
 
 notation SemiR (infixr ";" 140)
 
-subsection {* Evaluation Function *}
-
-definition BindR ::
-  "('VALUE, 'TYPE) BINDING \<Rightarrow>
-   ('VALUE, 'TYPE) RELATION" where
-"BindR b =
- {(rb1, rb2) . \<exists> b' \<in> WF_BINDING .
-   rb1 = b \<oplus> b' on DASHED \<and> rb2 = (SubstB SS b) \<oplus> b' on DASHED}"
-
-definition EvalR ::
-  "('VALUE, 'TYPE) PREDICATE \<Rightarrow>
-   ('VALUE, 'TYPE) RELATION" ("\<lbrakk>_\<rbrakk>R") where
-"EvalR p = \<Union> (BindR ` p)"
-
-definition IEvalR ::
-  "('VALUE, 'TYPE) RELATION \<Rightarrow>
-   ('VALUE, 'TYPE) PREDICATE" where
-"IEvalR rbs =
- {rb1 \<oplus> (SubstB SS rb2) on DASHED | rb1 rb2 . (rb1, rb2) \<in> rbs}"
-
 subsection {* Theorems *}
 
-subsubsection {* Theorems about @{term SS} *}
-
-text {* TODO: Maybe try and shorten the following proof. *}
-
-theorem SS_VAR_SUBST [closure] :
-"SS \<in> VAR_SUBST"
-apply (simp add: SS_def VAR_SUBST_def)
-apply (simp add: bij_def)
-apply (rule conjI)
-apply (simp add: inj_on_def)
-apply (safe)
-apply (auto)
-apply (insert dash_inj undash_inj_on_DASHED)
--- {* Subgoal 1 *}
-apply (simp add: inj_on_eq_iff)
--- {* Subgoal 2 *}
-apply (simp add: inj_eq)
--- {* Subgoal 3 *}
-apply (simp add: image_def)
-apply (drule_tac x = "dash x" in bspec) back
-apply (simp add: var_defs)
-apply (simp)
--- {* Subgoal 4 *}
-apply (simp add: image_def)
-apply (drule_tac x = "undash x" in bspec)
-apply (simp)
-apply (simp)
-done
-
-theorem SS_VAR_SUBST_ON [closure] :
-"SS \<in> VAR_SUBST_ON (UNDASHED \<union> DASHED)"
-apply (simp add: VAR_SUBST_ON_def)
-apply (simp add: SS_VAR_SUBST)
-apply (simp add: SS_def)
-done
-
-theorem SS_VAR_SUBST_INV [closure] :
-"SS \<in> VAR_SUBST_INV"
-apply (simp add: VAR_SUBST_INV_def)
-apply (simp add: SS_VAR_SUBST)
-apply (rule sym [OF inv_equality])
-apply (simp_all add: SS_def)
-apply (auto)
-done
-
-theorem SS_inv [simp] :
-"inv SS = SS"
-apply (insert SS_VAR_SUBST_INV)
-apply (simp add: VAR_SUBST_INV_def)
-done
-
 subsubsection {* Closure Theorems *}
+
+theorem SkipR_closure [closure] :
+"II \<in> WF_PREDICATE"
+apply (simp add: SkipR_def)
+apply (simp add: WF_PREDICATE_def)
+apply (auto)
+done
 
 theorem SemiR_closure [closure] :
 "\<lbrakk>p1 \<in> WF_PREDICATE;
@@ -127,265 +66,6 @@ theorem SemiR_closure [closure] :
 apply (simp add: SemiR_def)
 apply (simp add: WF_PREDICATE_def)
 apply (auto)
-done
-
-subsubsection {* Transfer Theorems *}
-
-lemma SS_DASHED_member :
-"x \<in> DASHED \<Longrightarrow> \<not> SS x \<in> DASHED"
-apply (simp add: SS_def)
-apply (simp add: var_defs)
-done
-
-lemma IEvalR_inverse_lemma1 :
-"\<lbrakk>b \<in> WF_BINDING;
- b' \<in> WF_BINDING\<rbrakk> \<Longrightarrow>
- b \<oplus> SubstB SS (SubstB SS b \<oplus> b' on DASHED) on DASHED = b"
-apply (rule ext)
-apply (case_tac "x \<in> DASHED")
-apply (simp_all add: SubstB_def SS_DASHED_member closure)
-done
-
-lemma IEvalR_inverse_lemma2 :
-"\<lbrakk>b \<in> WF_BINDING\<rbrakk> \<Longrightarrow>
- b \<oplus> SubstB SS (SubstB SS b \<oplus> b on DASHED) on DASHED = b"
-apply (rule ext)
-apply (case_tac "x \<in> DASHED")
-apply (simp_all add: SubstB_def SS_DASHED_member closure)
-done
-
-theorem IEvalR_inverse :
-"p \<in> WF_PREDICATE \<Longrightarrow> IEvalR (EvalR p) = p"
-apply (simp add: IEvalR_def EvalR_def)
-apply (safe)
--- {* Subgoal 1 *}
-apply (rename_tac bx rb1 rb2 b)
-apply (simp add: BindR_def)
-apply (clarsimp)
-apply (simp add: IEvalR_inverse_lemma1)
--- {* Subgoal 2 *}
-apply (rename_tac b)
-apply (rule_tac x = "b" in exI)
-apply (rule_tac x = "(SubstB SS b) \<oplus> b on DASHED" in exI)
-apply (rule conjI)
--- {* Subgoal 2.1 *}
-apply (simp add: IEvalR_inverse_lemma2)
--- {* Subgoal 2.2 *}
-apply (rule_tac x = "b" in bexI)
-apply (simp add: BindR_def)
-apply (rule_tac x = "b" in bexI)
-apply (simp_all)
-done
-
-theorem EvalR_inj :
-"inj_on EvalR WF_PREDICATE"
-apply (insert IEvalR_inverse)
-apply (erule inj_on_inverseI)
-done
-
-theorem EvalR_simp :
-"\<lbrakk>p1 \<in> WF_PREDICATE;
- p2 \<in> WF_PREDICATE\<rbrakk> \<Longrightarrow>
- p1 = p2 \<longleftrightarrow> \<lbrakk>p1\<rbrakk>R = \<lbrakk>p2\<rbrakk>R"
-apply (rule inj_on_eval_simp [of EvalR WF_PREDICATE "p1" "p2"])
-apply (simp add: EvalR_inj)
-apply (assumption)+
-done
-
-theorem EvalR_intro :
-"\<lbrakk>p1 \<in> WF_PREDICATE;
- p2 \<in> WF_PREDICATE;
- \<lbrakk>p1\<rbrakk>R = \<lbrakk>p2\<rbrakk>R\<rbrakk> \<Longrightarrow> p1 = p2"
-apply (rule inj_on_eval_intro [of EvalR WF_PREDICATE "p1" "p2"])
-apply (simp add: EvalR_inj)
-apply (assumption)+
-done
-
-subsubsection {* Evaluation Theorems *}
-
-theorem BindR_WF_BINDING_eq :
-"\<lbrakk>b1 \<in> WF_BINDING;
- b2 \<in> WF_BINDING;
- rb \<in> BindR b1;
- rb \<in> BindR b2\<rbrakk> \<Longrightarrow> b1 = b2"
-apply (simp add: BindR_def)
-apply (safe)
-apply (rename_tac x y b2' b1')
-apply (simp add: override_on_equals)
-apply (safe)
-apply (rule ext)
-apply (case_tac "x \<notin> DASHED")
--- {* Subgoal 1 *}
-apply (simp)
--- {* Subgoal 2 *}
-apply (clarsimp)
-apply (drule_tac x = "undash x" in spec)
-apply (subgoal_tac "undash x \<notin> DASHED")
-apply (simp)
-apply (simp add: SubstB_def closure)
-apply (simp add: SS_def)
-apply (simp add: var_defs)
-done
-
-theorem EvalR_NotP :
-"\<lbrakk>p \<in> WF_PREDICATE\<rbrakk> \<Longrightarrow>
- \<lbrakk>\<not>p p\<rbrakk>R = \<lbrakk>true\<rbrakk>R - \<lbrakk>p\<rbrakk>R"
-apply (simp add: EvalR_def)
-apply (simp add: NotP_def TrueP_def)
-apply (auto)
-apply (rename_tac rb b2 b1)
-apply (subgoal_tac "b1 = b2")
-apply (simp)
-apply (simp add: BindR_WF_BINDING_eq closure)
-done
-
-theorem EvalR_AndP :
-"\<lbrakk>p1 \<in> WF_PREDICATE;
- p2 \<in> WF_PREDICATE\<rbrakk> \<Longrightarrow>
- \<lbrakk>p1 \<and>p p2\<rbrakk>R = \<lbrakk>p1\<rbrakk>R \<inter> \<lbrakk>p2\<rbrakk>R"
-apply (simp add: EvalR_def)
-apply (simp add: AndP_def)
-apply (auto)
-apply (rename_tac b b1 b2)
-apply (rule_tac x = "b2" in bexI)
-apply (assumption)
-apply (subgoal_tac "b1 = b2")
-apply (simp)
-apply (simp add: BindR_WF_BINDING_eq closure)
-done
-
-theorem EvalR_OrP :
-"\<lbrakk>p1 \<in> WF_PREDICATE;
- p2 \<in> WF_PREDICATE\<rbrakk> \<Longrightarrow>
- \<lbrakk>p1 \<or>p p2\<rbrakk>R = \<lbrakk>p1\<rbrakk>R \<union> \<lbrakk>p2\<rbrakk>R"
-apply (simp add: EvalR_def)
-apply (simp add: OrP_def)
-done
-
-theorem SubstB_SS_COMPOSABLE_1 :
-"\<lbrakk>b1 \<in> WF_BINDING;
- b2 \<in> WF_BINDING;
- (b1, b2) \<in> COMPOSABLE; x \<notin> DASHED\<rbrakk> \<Longrightarrow>
- SubstB SS b1 x = b2 x"
-apply (simp add: SubstB_def closure)
-apply (simp add: SS_def)
-apply (safe)
-apply (simp add: COMPOSABLE_def)
-apply (simp add: COMPOSABLE_def)
-apply (clarify)
-apply (simp add: binding_equiv_def)
-apply (simp add: OTHER_VAR_def)
-apply (drule_tac x = "x" in bspec) back
-apply (simp add: VAR_def)
-apply (assumption)
-done
-
-theorem SubstB_SS_COMPOSABLE_2 :
-"\<lbrakk>b1 \<in> WF_BINDING;
- b2 \<in> WF_BINDING;
- (b1, b2) \<in> COMPOSABLE; x \<notin> DASHED\<rbrakk> \<Longrightarrow>
- SubstB SS (b1 \<oplus> b2 on DASHED) x = SubstB SS b2 x"
-apply (simp add: SubstB_def closure)
-apply (simp add: SS_def)
-apply (simp add: COMPOSABLE_def)
-apply (clarify)
-apply (simp add: binding_equiv_def)
-apply (simp add: OTHER_VAR_def)
-apply (drule_tac x = "x" in bspec) back
-apply (simp add: VAR_def)
-apply (assumption)
-done
-
-theorems SubstB_SS_COMPOSABLE =
-  SubstB_SS_COMPOSABLE_1
-  SubstB_SS_COMPOSABLE_2
-
-theorem BindR_COMPOSABLE :
-"\<lbrakk>b1 \<in> WF_BINDING;
- b2 \<in> WF_BINDING;
- (rb1, rb3) \<in> BindR b1;
- (rb3, rb2) \<in> BindR b2\<rbrakk> \<Longrightarrow>
- (b1, b2) \<in> COMPOSABLE"
-apply (simp add: BindR_def COMPOSABLE_def)
-apply (safe)
-apply (simp_all add: SubstB_def closure)
-apply (simp_all add: override_on_equals)
-apply (safe)
--- {* Subgoal 1 *}
-apply (simp add: SS_def)
-apply (drule_tac x = "v" in spec) back
-apply (simp)
-apply (subgoal_tac "v \<notin> DASHED")
-apply (simp)
-apply (auto) [1]
--- {* Subgoal 2 *}
-apply (simp add: binding_equiv_def)
-apply (simp add: OTHER_VAR_def)
-apply (safe)
-apply (simp add: SS_def)
-apply (drule_tac x = "x" in spec) back
-apply (simp)
-done
-
-theorem BindR_override :
-"\<lbrakk>b1 \<in> WF_BINDING;
- b2 \<in> WF_BINDING;
- (rb1, rb3) \<in> BindR b1;
- (rb3, rb2) \<in> BindR b2\<rbrakk> \<Longrightarrow>
- (rb1, rb2) \<in> BindR (b1 \<oplus> b2 on DASHED)"
-apply (frule BindR_COMPOSABLE [of b1 b2 rb1 rb3 rb2])
-apply (assumption)+
-apply (simp add: BindR_def)
-apply (safe)
-apply (rule_tac x = "b'a" in bexI)
-apply (simp add: override_on_equals)
-apply (clarify)
-apply (drule_tac x = "x" in spec) back
-apply (clarify)
-apply (simp add: SubstB_SS_COMPOSABLE_2)
-apply (assumption)
-done
-
-theorem EvalR_SemiR :
-"\<lbrakk>p1 \<in> WF_PREDICATE;
- p2 \<in> WF_PREDICATE\<rbrakk> \<Longrightarrow>
- \<lbrakk>p1 ; p2\<rbrakk>R = \<lbrakk>p1\<rbrakk>R O \<lbrakk>p2\<rbrakk>R"
-apply (simp add: EvalR_def)
-apply (simp add: SemiR_def)
-apply (simp add: rel_comp_def)
-apply (insert WF_BINDING_exists)
-apply (safe)
--- {* Subgoal 1 *}
-apply (simp_all)
-apply (rename_tac rb1 rb2 b1 b2)
-apply (rule_tac x = "(SubstB SS b1) \<oplus> rb1 on DASHED" in exI)
-apply (rule conjI)
--- {* Subgoal 1.1 *}
-apply (rule_tac x = "b1" in bexI)
-apply (simp add: BindR_def)
-apply (clarify)
-apply (rule_tac x = "b'" in bexI)
-apply (simp)
-apply (assumption)+
--- {* Subgoal 1.2 *}
-apply (rule_tac x = "b2" in bexI)
-apply (simp add: BindR_def)
-apply (clarify)
-apply (rule_tac x = "b'" in bexI)
-apply (simp add: override_on_equals)
-apply (simp add: SubstB_SS_COMPOSABLE)
-apply (assumption)+
--- {* Subgoal 2 *}
-apply (rename_tac rb1 rb2 rb3 b1 b2)
-apply (rule_tac x = "b1 \<oplus> b2 on DASHED" in exI)
-apply (rule conjI)
--- {* Subgoal 2.1 *}
-apply (rule_tac x = "b1" in exI)
-apply (rule_tac x = "b2" in exI)
-apply (simp)
-apply (simp add: BindR_COMPOSABLE)
--- {* Subgoal 2.1 *}
-apply (simp add: BindR_override)
 done
 
 subsection {* Proof Experiments *}
@@ -399,26 +79,7 @@ apply (subgoal_tac "(p1 ; p2) \<in> WF_PREDICATE")
 apply (subgoal_tac "(p2 ; p3) \<in> WF_PREDICATE")
 apply (simp add: SemiR_def)
 apply (safe)
-(* This is still fairly nasty! *)
+(* This is still quite nasty, even in the simplified predicate model! *)
 oops
-
-theorem SemiP_assoc :
-"\<lbrakk>p1 \<in> WF_PREDICATE;
- p2 \<in> WF_PREDICATE;
- p3 \<in> WF_PREDICATE\<rbrakk> \<Longrightarrow>
- (p1 ; p2) ; p3 = p1 ; (p2 ; p3)"
-apply (simp add: EvalR_simp closure)
-apply (simp add: EvalR_SemiR closure)
-apply (auto)
-done
-
-theorem SemiP_OrP_distr :
-"\<lbrakk>p1 \<in> WF_PREDICATE;
- p2 \<in> WF_PREDICATE;
- p3 \<in> WF_PREDICATE\<rbrakk> \<Longrightarrow>
- p1 ; (p2 \<or>p p3) = (p1 ; p2) \<or>p (p1 ; p3)"
-apply (simp add: EvalR_simp closure)
-apply (simp add: EvalR_SemiR EvalR_OrP closure)
-done
 end
 end
