theories/utils/utp_eval_rel.thy
@@ -1,0 +1,569 @@
+(******************************************************************************)
+(* Project: Unifying Theories of Programming                                  *)
+(* File: utp_rel_eval.thy                                                     *)
+(* Author: Frank Zeyda, University of York (UK)                               *)
+(******************************************************************************)
+
+header {* Proof Tactic for Relations *}
+
+theory utp_eval_rel
+imports "../generic/utp_pred" "../generic/utp_rel"
+begin
+
+text {* Theorem Attribute *}
+
+ML {*
+  structure evalr =
+    Named_Thms (val name = "evalr" val description = "evalr theorems")
+*}
+
+setup evalr.setup
+
+subsection {* Type Synonyms *}
+
+type_synonym ('VALUE, 'TYPE) RELATION =
+  "(('VALUE, 'TYPE) BINDING \<times>
+    ('VALUE, 'TYPE) BINDING) set"
+
+context PRED
+begin
+
+subsection {* Auxiliary Definitions *}
+
+text {*
+  We require an arbitrary but fixed binding in our model of relations in order
+  to constrain dashed variables which we do not care about. We note that an
+  alternative approach is possible that upward closes the relation with respect
+  to the values of these variables. In practice, it turns out that a constant
+  valuation yields simpler proofs and there is not loss of generality with it.
+*}
+
+definition bc :: "('VALUE, 'TYPE) BINDING" where
+"bc = (SOME b . b \<in> WF_BINDING)"
+
+theorem bc_WF_BINDING [closure] :
+"bc \<in> WF_BINDING"
+apply (simp add: bc_def)
+apply (rule_tac P = "\<lambda> b . b \<in> WF_BINDING" in someI_ex)
+apply (simp add: WF_BINDING_exists)
+done
+
+subsection {* Semantic Domain *}
+
+definition WF_REL_BINDING :: "('VALUE, 'TYPE) BINDING set" where
+"WF_REL_BINDING = {b \<oplus> bc on DASHED | b . b \<in> WF_BINDING}"
+
+subsection {* Interpretation Function *}
+
+text {* The substitution @{term "SS"} swaps dashed and undashed variables. *}
+
+definition SS :: "'TYPE VAR \<Rightarrow> 'TYPE VAR" where
+"SS = (\<lambda> v .
+   if v \<in> UNDASHED then (dash v) else
+   if v \<in> DASHED then (undash v) else v)"
+
+definition BindR ::
+  "('VALUE, 'TYPE) BINDING \<Rightarrow>
+   ('VALUE, 'TYPE) BINDING \<times>
+   ('VALUE, 'TYPE) BINDING" where
+"BindR b = (b \<oplus> bc on DASHED, (SubstB SS b) \<oplus> bc on DASHED)"
+
+definition BindP ::
+  "('VALUE, 'TYPE) BINDING \<times>
+   ('VALUE, 'TYPE) BINDING \<Rightarrow>
+   ('VALUE, 'TYPE) BINDING" where
+"BindP = (\<lambda> (rb1, rb2) . rb1 \<oplus> (SubstB SS rb2) on DASHED)"
+
+definition EvalR ::
+  "('VALUE, 'TYPE) PREDICATE \<Rightarrow>
+   ('VALUE, 'TYPE) RELATION" ("\<lbrakk>_\<rbrakk>R") where
+"EvalR p = BindR ` p"
+
+definition IEvalR ::
+  "('VALUE, 'TYPE) RELATION \<Rightarrow>
+   ('VALUE, 'TYPE) PREDICATE" where
+"IEvalR r = BindP ` r"
+
+subsection {* Theorems about @{term SS} *}
+
+text {* TODO: Maybe try and shorten the following proof. *}
+
+theorem SS_VAR_SUBST [closure] :
+"SS \<in> VAR_SUBST"
+apply (simp add: SS_def VAR_SUBST_def)
+apply (simp add: bij_def)
+apply (rule conjI)
+apply (simp add: inj_on_def)
+apply (safe)
+apply (auto)
+apply (insert dash_inj undash_inj_on_DASHED)
+-- {* Subgoal 1 *}
+apply (simp add: inj_on_eq_iff)
+-- {* Subgoal 2 *}
+apply (simp add: inj_eq)
+-- {* Subgoal 3 *}
+apply (simp add: image_def)
+apply (drule_tac x = "dash x" in bspec) back
+apply (simp add: var_defs)
+apply (simp)
+-- {* Subgoal 4 *}
+apply (simp add: image_def)
+apply (drule_tac x = "undash x" in bspec)
+apply (simp)
+apply (simp)
+done
+
+theorem SS_VAR_SUBST_ON [closure] :
+"SS \<in> VAR_SUBST_ON (UNDASHED \<union> DASHED)"
+apply (simp add: VAR_SUBST_ON_def)
+apply (simp add: SS_VAR_SUBST)
+apply (simp add: SS_def)
+done
+
+theorem SS_VAR_SUBST_INV [closure] :
+"SS \<in> VAR_SUBST_INV"
+apply (simp add: VAR_SUBST_INV_def)
+apply (simp add: SS_VAR_SUBST)
+apply (rule sym [OF inv_equality])
+apply (simp_all add: SS_def)
+apply (auto)
+done
+
+theorem SS_inv [simp] :
+"inv SS = SS"
+apply (insert SS_VAR_SUBST_INV)
+apply (simp add: VAR_SUBST_INV_def)
+done
+
+theorem SS_DASHED_member :
+"x \<in> DASHED \<Longrightarrow> \<not> SS x \<in> DASHED"
+apply (simp add: SS_def)
+apply (simp add: var_defs)
+done
+
+theorem SubstB_SS_COMPOSABLE_1 :
+"\<lbrakk>b1 \<in> WF_BINDING;
+ b2 \<in> WF_BINDING;
+ (b1, b2) \<in> COMPOSABLE\<rbrakk> \<Longrightarrow>
+ SubstB SS b1 \<oplus> bc on DASHED = b2 \<oplus> bc on DASHED"
+apply (simp add: override_on_equals)
+apply (simp add: SubstB_def closure)
+apply (simp add: SS_def)
+apply (safe)
+apply (simp add: COMPOSABLE_def)
+apply (simp add: COMPOSABLE_def)
+apply (clarify)
+apply (simp add: binding_equiv_def)
+apply (simp add: NON_REL_VAR_def)
+apply (drule_tac x = "x" in bspec) back
+apply (simp add: VAR_def)
+apply (assumption)
+done
+
+theorem SubstB_SS_COMPOSABLE_2 :
+"\<lbrakk>b1 \<in> WF_BINDING;
+ b2 \<in> WF_BINDING;
+ (b1, b2) \<in> COMPOSABLE\<rbrakk> \<Longrightarrow>
+ SubstB SS (b1 \<oplus> b2 on DASHED) \<oplus> bc on DASHED = SubstB SS b2 \<oplus> bc on DASHED"
+apply (simp add: override_on_equals)
+apply (simp add: SubstB_def closure)
+apply (simp add: SS_def)
+apply (safe)
+apply (simp add: COMPOSABLE_def)
+apply (clarify)
+apply (simp add: binding_equiv_def)
+apply (simp add: NON_REL_VAR_def)
+apply (drule_tac x = "x" in bspec) back
+apply (simp add: VAR_def)
+apply (assumption)
+done
+
+theorems SubstB_SS_COMPOSABLE =
+  SubstB_SS_COMPOSABLE_1
+  SubstB_SS_COMPOSABLE_2
+
+subsection {* Model Theorems *}
+
+theorem EvalR_range :
+"p \<in> WF_PREDICATE \<Longrightarrow>
+ \<lbrakk>p\<rbrakk>R \<subseteq> WF_REL_BINDING \<times> WF_REL_BINDING"
+apply (simp add: EvalR_def)
+apply (simp add: image_def)
+apply (simp add: BindR_def)
+apply (simp add: WF_REL_BINDING_def)
+apply (safe)
+apply (rule_tac x = "xa" in exI)
+apply (simp)
+apply (rule_tac x = "SubstB SS xa" in exI)
+apply (simp add: closure)
+done
+
+theorem WF_REL_BINDING_member1 [simp, intro] :
+"\<lbrakk>p \<in> WF_PREDICATE;
+ (rb1, rb2) \<in> \<lbrakk>p\<rbrakk>R\<rbrakk> \<Longrightarrow>
+ rb1 \<in> WF_REL_BINDING"
+apply (auto dest: EvalR_range)
+done
+
+theorem WF_REL_BINDING_member2 [simp, intro] :
+"\<lbrakk>p \<in> WF_PREDICATE;
+ (rb1, rb2) \<in> \<lbrakk>p\<rbrakk>R\<rbrakk> \<Longrightarrow>
+ rb2 \<in> WF_REL_BINDING"
+apply (auto dest: EvalR_range)
+done
+
+theorem BindP_inverse :
+"b \<in> WF_BINDING \<Longrightarrow> BindP (BindR b) = b"
+apply (simp add: BindR_def BindP_def)
+apply (rule ext)
+apply (case_tac "x \<in> DASHED")
+apply (simp add: SubstB_def SS_DASHED_member closure)
+apply (simp)
+done
+
+theorem BindR_inject [simp] :
+"\<lbrakk>b1 \<in> WF_BINDING;
+ b2 \<in> WF_BINDING\<rbrakk> \<Longrightarrow>
+ BindR b1 = BindR b2 \<longleftrightarrow> b1 = b2"
+apply (simp add: BindR_def)
+apply (simp add: override_on_equals)
+apply (safe)
+apply (rule ext)
+apply (case_tac "x \<in> DASHED")
+-- {* Subgoal 1 *}
+apply (drule_tac x = "undash x" in spec)
+back
+apply (subgoal_tac "undash x \<notin> DASHED")
+apply (simp)
+apply (simp add: SubstB_def closure)
+apply (simp add: SS_def)
+apply (simp add: var_defs)
+-- {* Subgoal 2 *}
+apply (simp)
+done
+
+theorem BindR_COMPOSABLE :
+"\<lbrakk>b1 \<in> WF_BINDING;
+ b2 \<in> WF_BINDING;
+ (rb1, rb3) = BindR b1;
+ (rb3, rb2) = BindR b2\<rbrakk> \<Longrightarrow>
+ (b1, b2) \<in> COMPOSABLE"
+apply (simp add: BindR_def COMPOSABLE_def)
+apply (simp add: override_on_equals)
+apply (simp_all add: SubstB_def closure)
+apply (safe)
+-- {* Subgoal 1 *}
+apply (simp add: SS_def)
+apply (drule_tac x = "v" in spec)
+apply (simp)
+apply (auto) [1]
+-- {* Subgoal 2 *}
+apply (simp add: binding_equiv_def)
+apply (simp add: NON_REL_VAR_def)
+apply (safe)
+apply (simp add: SS_def)
+apply (drule_tac x = "x" in spec)
+apply (simp)
+done
+
+theorem BindR_override :
+"\<lbrakk>b1 \<in> WF_BINDING;
+ b2 \<in> WF_BINDING;
+ (rb1, rb3) = BindR b1;
+ (rb3, rb2) = BindR b2\<rbrakk> \<Longrightarrow>
+ (rb1, rb2) = BindR (b1 \<oplus> b2 on DASHED)"
+apply (simp add: BindR_def)
+apply (simp add: override_on_equals)
+apply (simp_all add: SubstB_def closure)
+apply (clarify)
+apply (simp add: SS_def)
+apply (safe)
+apply (drule_tac x = "x" in spec)
+apply (simp)
+done
+
+theorem IEvalR_inverse :
+"p \<in> WF_PREDICATE \<Longrightarrow> IEvalR (EvalR p) = p"
+apply (simp add: IEvalR_def EvalR_def)
+apply (simp add: image_image)
+apply (simp add: image_def)
+apply (simp add: set_eq_iff)
+apply (simp add: BindP_inverse)
+done
+
+subsection {* Transfer Theorems *}
+
+theorem EvalR_inj_on :
+"inj_on EvalR WF_PREDICATE"
+apply (insert IEvalR_inverse)
+apply (erule inj_on_inverseI)
+done
+
+theorem EvalR_simp [evalr] :
+"\<lbrakk>p1 \<in> WF_PREDICATE;
+ p2 \<in> WF_PREDICATE\<rbrakk> \<Longrightarrow>
+ p1 = p2 \<longleftrightarrow> \<lbrakk>p1\<rbrakk>R = \<lbrakk>p2\<rbrakk>R"
+apply (rule inj_on_eval_simp [of EvalR WF_PREDICATE "p1" "p2"])
+apply (simp add: EvalR_inj_on)
+apply (assumption)+
+done
+
+theorem EvalR_intro :
+"\<lbrakk>p1 \<in> WF_PREDICATE;
+ p2 \<in> WF_PREDICATE;
+ \<lbrakk>p1\<rbrakk>R = \<lbrakk>p2\<rbrakk>R\<rbrakk> \<Longrightarrow> p1 = p2"
+apply (rule inj_on_eval_intro [of EvalR WF_PREDICATE "p1" "p2"])
+apply (simp add: EvalR_inj_on)
+apply (assumption)+
+done
+
+subsection {* Distribution Theorems *}
+
+theorem EvalR_TrueP_explicit :
+"\<lbrakk>true\<rbrakk>R = {(b1, b2) | b1 b2 .
+   b1 \<in> WF_REL_BINDING \<and>
+   b2 \<in> WF_REL_BINDING \<and>
+   b1 \<cong> b2 on DASHED \<and>
+   b1 \<cong> b2 on NON_REL_VAR}"
+apply (simp add: EvalR_def)
+apply (simp add: TrueP_def)
+apply (simp add: image_def)
+apply (simp add: BindR_def WF_REL_BINDING_def)
+apply (simp add: binding_equiv_def)
+apply (simp add: set_eq_subset)
+apply (safe)
+-- {* Subgoal 1 *}
+apply (rule_tac x = "xa" in exI)
+apply (simp)
+-- {* Subgoal 2 *}
+apply (rule_tac x = "SubstB SS xa" in exI)
+apply (simp add: closure)
+-- {* Subgoal 3 *}
+apply (simp)
+-- {* Subgoal 4 *}
+apply (simp add: NON_REL_VAR_def)
+apply (simp add: SubstB_def closure)
+apply (simp add: SS_def)
+-- {* Subgoal 5 *}
+apply (rule_tac x = "b \<oplus> (SubstB SS ba) on DASHED" in bexI)
+apply (simp)
+apply (simp add: override_on_equals)
+apply (safe)
+apply (simp add: SubstB_def closure)
+apply (simp add: SS_def)
+apply (auto) [1]
+apply (drule_tac x = "x" in bspec)
+apply (simp add: NON_REL_VAR_def var_defs)
+apply (simp)
+apply (simp add: closure)
+done
+
+theorem EvalR_TrueP [evalr] :
+"\<lbrakk>true\<rbrakk>R = \<lbrakk>WF_BINDING\<rbrakk>R"
+apply (simp add: EvalR_def)
+apply (simp add: TrueP_def)
+done
+
+theorem EvalR_FalseP [evalr] :
+"\<lbrakk>false\<rbrakk>R = {}"
+apply (simp add: EvalR_def)
+apply (simp add: FalseP_def)
+done
+
+theorem EvalR_NotP [evalr] :
+"\<lbrakk>p \<in> WF_PREDICATE\<rbrakk> \<Longrightarrow>
+ \<lbrakk>\<not>p p\<rbrakk>R = \<lbrakk>true\<rbrakk>R - \<lbrakk>p\<rbrakk>R"
+apply (simp add: EvalR_def)
+apply (simp add: NotP_def TrueP_def)
+apply (auto)
+done
+
+theorem EvalR_AndP [evalr] :
+"\<lbrakk>p1 \<in> WF_PREDICATE;
+ p2 \<in> WF_PREDICATE\<rbrakk> \<Longrightarrow>
+ \<lbrakk>p1 \<and>p p2\<rbrakk>R = \<lbrakk>p1\<rbrakk>R \<inter> \<lbrakk>p2\<rbrakk>R"
+apply (simp add: EvalR_def)
+apply (simp add: AndP_def)
+apply (auto)
+done
+
+theorem EvalR_OrP [evalr] :
+"\<lbrakk>p1 \<in> WF_PREDICATE;
+ p2 \<in> WF_PREDICATE\<rbrakk> \<Longrightarrow>
+ \<lbrakk>p1 \<or>p p2\<rbrakk>R = \<lbrakk>p1\<rbrakk>R \<union> \<lbrakk>p2\<rbrakk>R"
+apply (simp add: EvalR_def)
+apply (simp add: OrP_def)
+apply (auto)
+done
+
+declare ImpliesP_def [evalr]
+
+declare IffP_def [evalr]
+
+theorem EvalR_SkipR [evalr] :
+"\<lbrakk>II\<rbrakk>R = Id_on WF_REL_BINDING"
+apply (simp add: EvalR_def)
+apply (simp add: SkipR_def)
+apply (simp add: WF_REL_BINDING_def)
+apply (simp add: image_def)
+apply (simp add: BindR_def)
+apply (simp add: Id_on_def)
+apply (simp add: set_eq_iff)
+apply (safe)
+-- {* Subgoal 1 *}
+apply (rename_tac x b)
+apply (rule_tac x = "b \<oplus> bc on DASHED" in exI)
+apply (simp add: override_on_equals)
+apply (rule conjI)
+apply (rule_tac x = "b" in exI)
+apply (simp)
+apply (simp add: SubstB_def closure)
+apply (simp add: SS_def)
+-- {* Subgoal 2 *}
+apply (rule_tac x = "b \<oplus> (SubstB SS b) on DASHED" in exI)
+apply (simp add: override_on_equals)
+apply (simp add: closure)
+apply (rule conjI)
+-- {* Subgoal 2.1 *}
+apply (clarify)
+apply (subgoal_tac "v \<notin> DASHED")
+apply (simp)
+apply (simp add: SubstB_def closure)
+apply (simp add: SS_def)
+apply (auto) [1]
+apply (auto) [1]
+-- {* Subgoal 2.2 *}
+apply (simp add: SubstB_def closure)
+apply (simp add: SS_def)
+apply (auto) [1]
+done
+
+theorem EvalR_SemiR [evalr] :
+"\<lbrakk>p1 \<in> WF_PREDICATE;
+ p2 \<in> WF_PREDICATE\<rbrakk> \<Longrightarrow>
+ \<lbrakk>p1 ; p2\<rbrakk>R = \<lbrakk>p1\<rbrakk>R O \<lbrakk>p2\<rbrakk>R"
+apply (simp add: EvalR_def)
+apply (simp add: SemiR_def)
+apply (simp add: set_eq_iff)
+apply (simp add: rel_comp_def image_def)
+apply (safe)
+-- {* Subgoal 1 *}
+apply (rename_tac x rb1 rb2 xa b1 b2)
+apply (rule_tac x = "(SubstB SS b1) \<oplus> bc on DASHED" in exI)
+apply (rule conjI)
+-- {* Subgoal 1.1 *}
+apply (rule_tac x = "b1" in bexI)
+apply (simp add: BindR_def)
+apply (assumption)
+-- {* Subgoal 1.2 *}
+apply (rule_tac x = "b2" in bexI)
+apply (simp add: BindR_def)
+apply (simp add: SubstB_SS_COMPOSABLE)
+apply (assumption)
+-- {* Subgoal 2 *}
+apply (rename_tac x rb1 rb2 rb3 b1 b2)
+apply (rule_tac x = "b1 \<oplus> b2 on DASHED" in exI)
+apply (rule conjI)
+-- {* Subgoal 2.1 *}
+apply (rule_tac x = "b1" in exI)
+apply (rule_tac x = "b2" in exI)
+apply (simp)
+apply (simp add: BindR_COMPOSABLE)
+-- {* Subgoal 2.1 *}
+apply (simp add: BindR_override)
+done
+
+(* The following are useless since quantifications are not supported yet. *)
+
+(*
+declare Tautology_def [evalr]
+declare Contradiction_def [evalr]
+declare Refinement_def [evalr]
+*)
+end
+
+subsection {* Proof Tactics *}
+
+ML {*
+  fun utp_rel_simpset ctxt =
+    (simpset_of ctxt)
+      addsimps (evalr.get ctxt)
+      addsimps (closure.get ctxt);
+*}
+
+ML {*
+  fun utp_rel_auto_simpset ctxt =
+    (simpset_of ctxt)
+      addsimps @{thms "rel_comp_def"}
+*}
+
+ML {*
+  fun utp_rel_tac thms ctxt i =
+    CHANGED (asm_full_simp_tac (utp_rel_simpset ctxt) i)
+*}
+
+ML {*
+  fun utp_rel_auto_tac thms ctxt i =
+    TRY (asm_full_simp_tac (utp_rel_simpset ctxt) i) THEN
+    TRY (asm_full_simp_tac (utp_rel_auto_simpset ctxt) i) THEN
+    (auto_tac ctxt)
+*}
+
+method_setup utp_rel_tac = {*
+  Attrib.thms >>
+  (fn thms => fn ctxt =>
+    SIMPLE_METHOD' (utp_rel_tac thms ctxt))
+*} "proof tactic for relations"
+
+method_setup utp_rel_auto_tac = {*
+  Attrib.thms >>
+  (fn thms => fn ctxt =>
+    SIMPLE_METHOD' (utp_rel_auto_tac thms ctxt))
+*} "proof tactic for relations with auto"
+
+subsection {* Algebraic Laws *}
+
+context PRED
+begin
+theorem SemiP_FalseP :
+"\<lbrakk>p \<in> WF_PREDICATE\<rbrakk> \<Longrightarrow>
+ p ; false = false"
+apply (utp_rel_auto_tac)
+done
+
+theorem SemiP_OrP_distr :
+"\<lbrakk>p1 \<in> WF_PREDICATE;
+ p2 \<in> WF_PREDICATE;
+ p3 \<in> WF_PREDICATE\<rbrakk> \<Longrightarrow>
+ p1 ; (p2 \<or>p p3) = (p1 ; p2) \<or>p (p1 ; p3)"
+apply (utp_rel_auto_tac)
+done
+
+theorem SemiP_IffP_comm :
+"\<lbrakk>p1 \<in> WF_PREDICATE;
+ p2 \<in> WF_PREDICATE\<rbrakk> \<Longrightarrow>
+ p1 \<Leftrightarrow>p p2 = p2 \<Leftrightarrow>p p1"
+apply (utp_rel_auto_tac)
+done
+
+theorem SemiP_SkipR_left :
+"\<lbrakk>p \<in> WF_PREDICATE\<rbrakk> \<Longrightarrow>
+ II ; p = p"
+apply (utp_rel_auto_tac)
+done
+
+theorem SemiP_SkipR_right :
+"\<lbrakk>p \<in> WF_PREDICATE\<rbrakk> \<Longrightarrow>
+ p ; II = p"
+apply (utp_rel_auto_tac)
+done
+
+theorem SemiP_assoc :
+"\<lbrakk>p1 \<in> WF_PREDICATE;
+ p2 \<in> WF_PREDICATE;
+ p3 \<in> WF_PREDICATE\<rbrakk> \<Longrightarrow>
+ (p1 ; p2) ; p3 = p1 ; (p2 ; p3)"
+apply (utp_rel_auto_tac)
+done
+end
+end
